theories/ftlr/interp_weakening.v
@@ -6,21 +6,23 @@ From cap_machine Require Export logrel ftlr_base.
 
 Section fundamental.
   Context
-    {Σ : gFunctors}
-      {ceriseg: ceriseG Σ}
-      {stsg : STSG Addr region_type Σ} {heapg : heapGS Σ}
-      {sealsg: sealStoreG Σ}
-      {nainv: logrel_na_invs Σ}
-      {MP: MachineParameters}
-  .
+    {Σ:gFunctors}
+    {ceriseg:ceriseG Σ} {sealsg: sealStoreG Σ}
+    {Cname : CmptNameG}
+    {stsg : STSG Addr region_type Σ} {heapg : heapGS Σ}
+    {nainv: logrel_na_invs Σ}
+    `{MP: MachineParameters}.
 
   Notation STS := (leibnizO (STS_states * STS_rels)).
   Notation STS_STD := (leibnizO (STS_std_states Addr region_type)).
-  Notation WORLD := (prodO STS_STD STS).
+  Notation CVIEW := (prodO STS_STD STS).
+  Notation WORLD := (gmapO CmptName CVIEW).
+  Implicit Types WC : CVIEW.
   Implicit Types W : WORLD.
+  Implicit Types C : CmptName.
 
-  Notation D := (WORLD -n> (leibnizO Word) -n> iPropO Σ).
-  Notation R := (WORLD -n> (leibnizO Reg) -n> iPropO Σ).
+  Notation D := (WORLD -n> (leibnizO CmptName) -n> (leibnizO Word) -n> iPropO Σ).
+  Notation R := (WORLD -n> (leibnizO CmptName) -n> (leibnizO Reg) -n> iPropO Σ).
   Implicit Types w : (leibnizO Word).
   Implicit Types interp : (D).
 
